\documentclass{article}
\usepackage[utf8]{inputenc}

\title{EE3900-assign1}
\author{VEERAVALLI BHANU PRAKASH}
\date{August 2022}

\begin{document}

\maketitle

\section{4.2 solution}
$$x(n)={\{1, 2, 3, 4, 2, 1\}}$$
$$X(z)=Z\{x(n)\}=\sum_{0}^{5}x(n)*(z^{-n}))$$
$$X(z)=1*z^{0}+2*Z^{-1}+3*z^{-2}+4*z^{-3}+2*z^{-4}+1*z^{-5}$$
\section{4.5 solution}
$$y=a^nu(n)$$
$$u(n)=
\left\{
	\begin{array}{ll}
		1 & \mbox{if } n \geq 0 \\
		0 & \mbox{if } n < 0
	\end{array}
\right.$$
$$a^nu(n)=
\left\{
	\begin{array}{ll}
		a^n & \mbox{if } n \geq 0 \\
		0 & \mbox{if } n < 0
	\end{array}
\right.$$
$$Z{\{a^nu(n)\}}=\sum_{-\infty}^{\infty}a^nu(n)z^{-n}$$
$$Z{\{a^nu(n)\}}=\sum_{0}^{\infty}a^nz^{-n}$$
$$Z{\{a^nu(n)\}}=\sum_{0}^{\infty}{\frac{a}{z}}^n$$
$$ if \quad|z|>|a|\quad then \quad sum \quad of \quad G.P$$
$$Z{\{a^nu(n)\}}=\frac{1}{1-{az^{-1}}}$$
\section{5.1 solution }
\begin{equation}
    h(n) , n<5
\end{equation}

\begin{equation}
    H(z) = \frac{1 + z^{-2}}{1 + \frac{1}{2}z^{-1}}
\end{equation}
\begin{center}
    $1 + \frac{1}{2}z^{-1}\overline{)1 + z^{-2}(} 2z^{-1}$\\
    ${2z^{-1} + z^{-2}}$\\
    $1 + \frac{1}{2}z^{-1}\overline{)1-2z^{-1}(} -4$\\
    $-4 - 2z^{-1}$\\
    $\overline{5 + 0z^{-1}}$
\end{center}
Hence by long division will be 
\begin{equation}
    H(z) = 2z^{-1} -4 + \frac{5}{1 + \frac{1}{2}z^{-1}}
\end{equation}
\section{5.3 solution}
From the graph we can say that maximim value of h(n) is 1.25. 
The minimum value of graph is around -0.6.
$$-0.6 >h(n)\geq.25$$
The function is bounded between 1.25 and -0.6.
\section{5.4 solution}
$$h(n)=\bigg(-\frac{1}{2}\bigg)^nu(n)+\bigg(-\frac{1}{2}\bigg)^{n-2}u(n-2)$$
Ratio test
$$L=\lim_{n\to\infty} \bigg|\frac{h(n+1)}{h(n)}\bigg|$$
$$h(n+1)=\bigg(-\frac{1}{2}\bigg)^{n+1}u(n+1)+\bigg(-\frac{1}{2}\bigg)^{n-1}u(n-1)$$
$$h(n)=\bigg(-\frac{1}{2}\bigg)^nu(n)+\bigg(-\frac{1}{2}\bigg)^{n-2}u(n-2)$$
$$ as \quad n \rightarrow \infty \qquad u(n)=u(n-1)=u(n+1)=u(n-2)=1$$
$$h(n+1)={\{-\frac{1}{2}}\}{h(n)}$$
$$\bigg|\frac{h(n+1)}{h(n)}\bigg|=\bigg|-\frac{1}{2}\bigg|=\frac{1}{2}$$
$$L=\lim_{n\to\infty} \bigg|\frac{h(n+1)}{h(n)}\bigg|=\frac{1}{2}$$
L is less than 1 h(n) is convergent
\section{5.5 solution}
$$h(n)=\bigg(-\frac{1}{2}\bigg)^nu(n)+\bigg(-\frac{1}{2}\bigg)^{n-2}u(n-2)$$
$$\sum_{n=-\infty}^{\infty}h(n)=\sum_{n=-\infty}^{\infty}\bigg(-\frac{1}{2}\bigg)^nu(n)+\sum_{n=-\infty}^{\infty}\bigg(-\frac{1}{2}\bigg)^{n-2}u(n-2)$$
$$\sum_{n=-\infty}^{\infty}h(n)=\sum_{n=0}^{\infty}\bigg(-\frac{1}{2}\bigg)^nu(n)+\sum_{n=2}^{\infty}\bigg(-\frac{1}{2}\bigg)^{n-2}u(n-2)$$
$$\sum_{n=-\infty}^{\infty}h(n)=\sum_{n=0}^{\infty}\bigg(-\frac{1}{2}\bigg)^n+\sum_{n=2}^{\infty}\bigg(-\frac{1}{2}\bigg)^{n-2}$$
$$\sum_{n=-\infty}^{\infty}h(n)=\frac{4}{3}$$
\section{5.6}
\section{5.9 solution}
\section{5.10 solution}
from 5.13 we know that
$$y(n)=\sum_{k=-\infty}^{\infty}x(k)h(n-k)$$
$$t=n-k$$

$$y(n)=\sum_{n-t=-\infty}^{\infty}x(n-t)h(t) $$
since n is finite 
$$-\infty<\infty$$
the above equation is equivalet to
$$y(n)=\sum_{n=-\infty}^{\infty}x(n-t)h(t) $$
hence proved
\section{6.1 solution}

\end{document}
